MPPA - Oshrximm + Mgetparam + FP is GPR10 + bug
Added Oshrximm and Mgetparam -> mmult.c divide & conqueer generates

FP is now GPR10 instead of being a mix of GPR30 and GPR32

Corrected a bug where Pgoto and Pj_l were given the same interpretation,
where in fact there's a fundamental difference : Pgoto is supposed to
have a function name (symbol), while Pj_l is supposed to have a label
name (print_label). This led to having undefinite labels in the code.

mppa_k1c/TargetPrinter.ml
@@ -191,7 +191,9 @@ module Target : TARGET =
     let print_instruction oc = function
       | Pcall(s) ->
          fprintf oc "	call	%a\n;;\n" symbol s
-      | Pgoto(s) | Pj_l(s) ->
+      | Pgoto(s) ->
+         fprintf oc "	goto	%a\n;;\n" symbol s
+      | Pj_l(s) ->
          fprintf oc "	goto	%a\n;;\n" print_label s
       | Pret ->
          fprintf oc "	ret\n;;\n"
