test/mppa/mmult/mmult.c
@@ -39,7 +39,7 @@ typedef struct mblock {
 #define MAT_XY(mat, x, y) (mat)[(x)*SIZE + (y)]
 #define MAT_IJ(block, i, j) MAT_XY((block)->mat, (block)->imin + (i), block->jmin + (j))
 
-int strassen_mul(mblock *C, const mblock *A, const mblock *B){
+void divac_mul(mblock *C, const mblock *A, const mblock *B){
     const int size = C->imax - C->imin;
 
     for (int i = 0 ; i < size ; i++)
@@ -67,50 +67,50 @@ int strassen_mul(mblock *C, const mblock *A, const mblock *B){
         newb.jmax = (block)->jmax;\
     }
 
-int strassen_part(mblock *C, const mblock *A, const mblock *B);
+void divac_part(mblock *C, const mblock *A, const mblock *B);
 
-void strassen_wrap(mblock *C      , char IC, char JC,
+void divac_wrap(mblock *C      , char IC, char JC,
                    const mblock *A, char IA, char JA,
                    const mblock *B, char IB, char JB){
     MAKE_MBLOCK(Cb, C, IC, JC);
     MAKE_MBLOCK(Ab, A, IA, JA);
     MAKE_MBLOCK(Bb, B, IB, JB);
 
-    strassen_part(&Cb, &Ab, &Bb);
+    divac_part(&Cb, &Ab, &Bb);
 }
 
 
-int strassen_part(mblock *C, const mblock *A, const mblock *B){
+void divac_part(mblock *C, const mblock *A, const mblock *B){
     const int size = C->imax - C->imin;
 
     if (size % 2 == 1)
-        strassen_mul(C, A, B);
+        divac_mul(C, A, B);
     else{
         /* C_00 = A_00 B_00 + A_01 B_10 */
-        strassen_wrap(C, 0, 0, A, 0, 0, B, 0, 0);
-        strassen_wrap(C, 0, 0, A, 0, 1, B, 1, 0);
+        divac_wrap(C, 0, 0, A, 0, 0, B, 0, 0);
+        divac_wrap(C, 0, 0, A, 0, 1, B, 1, 0);
 
         /* C_10 = A_10 B_00 + A_11 B_10 */
-        strassen_wrap(C, 1, 0, A, 1, 0, B, 0, 0);
-        strassen_wrap(C, 1, 0, A, 1, 1, B, 1, 0);
+        divac_wrap(C, 1, 0, A, 1, 0, B, 0, 0);
+        divac_wrap(C, 1, 0, A, 1, 1, B, 1, 0);
 
         /* C_01 = A_00 B_01 + A_01 B_11 */
-        strassen_wrap(C, 0, 1, A, 0, 0, B, 0, 1);
-        strassen_wrap(C, 0, 1, A, 0, 1, B, 1, 1);
+        divac_wrap(C, 0, 1, A, 0, 0, B, 0, 1);
+        divac_wrap(C, 0, 1, A, 0, 1, B, 1, 1);
 
         /* C_11 = A_10 B_01 + A_11 B_11 */
-        strassen_wrap(C, 1, 1, A, 1, 0, B, 0, 1);
-        strassen_wrap(C, 1, 1, A, 1, 1, B, 1, 1);
+        divac_wrap(C, 1, 1, A, 1, 0, B, 0, 1);
+        divac_wrap(C, 1, 1, A, 1, 1, B, 1, 1);
     }
     
 }
 
-void mmult_strassen(uint64_t C[][SIZE], uint64_t A[][SIZE], uint64_t B[][SIZE]){
+void mmult_divac(uint64_t C[][SIZE], uint64_t A[][SIZE], uint64_t B[][SIZE]){
     mblock Cb = {.mat = (uint64_t *) C, .imin = 0, .imax = SIZE, .jmin = 0, .jmax = SIZE};
     mblock Ab = {.mat = (uint64_t *) A , .imin = 0, .imax = SIZE, .jmin = 0, .jmax = SIZE};
     mblock Bb = {.mat = (uint64_t *) B , .imin = 0, .imax = SIZE, .jmin = 0, .jmax = SIZE};
 
-    strassen_part(&Cb, &Ab, &Bb);
+    divac_part(&Cb, &Ab, &Bb);
 }
 
 #ifdef __UNIT_TEST_MMULT__
@@ -128,7 +128,7 @@ int main(void){
 
     mmult_row(C1, A, B);
     mmult_col(C2, A, B);
-    mmult_strassen(C3, A, B);
+    mmult_divac(C3, A, B);
 
     for (int i = 0 ; i < SIZE ; i++)
         for (int j = 0 ; j < SIZE ; j++)
