mppa_k1c/Asm.v
@@ -92,6 +92,7 @@ Module Pregmap := EMap(PregEq).
 (** Conventional names for stack pointer ([SP]) and return address ([RA]). *)
 
 Notation "'SP'" := GPR12 (only parsing) : asm.
+Notation "'FP'" := GPR10 (only parsing) : asm.
 Notation "'RTMP'" := GPR31 (only parsing) : asm.
 
 Inductive btest: Type :=
@@ -1008,7 +1009,7 @@ Definition exec_instr (f: function) (i: instruction) (rs: regset) (m: mem) : out
       let sp := (Vptr stk Ptrofs.zero) in
       match Mem.storev Mptr m1 (Val.offset_ptr sp pos) rs#SP with
       | None => Stuck
-      | Some m2 => Next (nextinstr (rs #GPR32 <- (rs SP) #SP <- sp #GPR31 <- Vundef)) m2
+      | Some m2 => Next (nextinstr (rs #FP <- (rs SP) #SP <- sp #GPR31 <- Vundef)) m2
       end
   | Pfreeframe sz pos =>
       match Mem.loadv Mptr m (Val.offset_ptr rs#SP pos) with
@@ -1082,7 +1083,7 @@ Definition preg_of (r: mreg) : preg :=
   match r with
   | R0  => GPR0  | R1  => GPR1  | R2  => GPR2  | R3  => GPR3  | R4  => GPR4
   | R5  => GPR5  | R6  => GPR6  | R7  => GPR7                 | R9  => GPR9
-(*| R10 => GPR10 | R11 => GPR11 | R12 => GPR12 | R13 => GPR13 | R14  => GPR14 *)
+  | R10 => GPR10 (*| R11 => GPR11 | R12 => GPR12 | R13 => GPR13 | R14  => GPR14 *)
   | R15 => GPR15 | R16 => GPR16 | R17 => GPR17 | R18 => GPR18 | R19  => GPR19
   | R20 => GPR20 | R21 => GPR21 | R22 => GPR22 | R23 => GPR23 | R24  => GPR24
   | R25 => GPR25 | R26 => GPR26 | R27 => GPR27 | R28 => GPR28 | R29  => GPR29
