mppa_k1c/Asmgenproof1.v
@@ -1214,6 +1214,18 @@ Opaque Int.eq.
 - (* Oaddrstack *)
   exploit addptrofs_correct. instantiate (1 := GPR12); auto with asmgen. intros (rs' & A & B & C).
   exists rs'; split; eauto. auto with asmgen.
+- (* Oshrximm *)
+  clear H. exploit Val.shrx_shr_2; eauto. intros E; subst v; clear EV.
+  destruct (Int.eq n Int.zero).
++ econstructor; split. apply exec_straight_one. simpl; eauto. auto.
+  split; intros; Simpl. 
++ change (Int.repr 32) with Int.iwordsize. set (n' := Int.sub Int.iwordsize n).
+  econstructor; split.
+  eapply exec_straight_step. simpl; reflexivity. auto. 
+  eapply exec_straight_step. simpl; reflexivity. auto. 
+  eapply exec_straight_step. simpl; reflexivity. auto. 
+  apply exec_straight_one. simpl; reflexivity. auto. 
+  split; intros; unfold getw; Simpl.
 - (* Ocast32signed *)
   exploit cast32signed_correct; eauto. intros (rs' & A & B & C).
   exists rs'; split; eauto. split. apply B.
@@ -1275,18 +1287,7 @@ Opaque Int.eq.
   exploit (opimm32_correct Pxorw Pxoriw Val.xor); auto. instantiate (1 := x0); eauto with asmgen.
   intros (rs' & A & B & C).
   exists rs'; split; eauto. rewrite B; auto with asmgen.
-- (* shrximm *)
-  clear H. exploit Val.shrx_shr_2; eauto. intros E; subst v; clear EV.
-  destruct (Int.eq n Int.zero).
-+ econstructor; split. apply exec_straight_one. simpl; eauto. auto.
-  split; intros; Simpl. 
-+ change (Int.repr 32) with Int.iwordsize. set (n' := Int.sub Int.iwordsize n).
-  econstructor; split.
-  eapply exec_straight_step. simpl; reflexivity. auto. 
-  eapply exec_straight_step. simpl; reflexivity. auto. 
-  eapply exec_straight_step. simpl; reflexivity. auto. 
-  apply exec_straight_one. simpl; reflexivity. auto. 
-  split; intros; Simpl.
+
 - (* longofintu *)
   econstructor; split.
   eapply exec_straight_three. simpl; eauto. simpl; eauto. simpl; eauto. auto. auto. auto.
